Define the logical relation...

UVal/UVal.v
@@ -21,42 +21,40 @@ Proof.
   induction n; eauto using Typing.
 Qed.
 
-Definition inUnit (n : nat) : Tm := abs tunit (inr (inl (var 0))).
+Definition inUnit (n : nat) (t : Tm) := inr (inl t).
 
-Lemma inUnitT {Γ n} : ⟪ Γ ⊢ inUnit n : tunit ⇒ UVal (S n) ⟫.
+Lemma inUnitT {Γ n t} : ⟪ Γ ⊢ t : tunit ⟫ → ⟪ Γ ⊢ inUnit n t : UVal (S n) ⟫.
 Proof.
+  intros tt.
   unfold inUnit. crushTyping.
 Qed.
 
-Definition inBool (n : nat) : Tm := abs tbool (inr (inr (inl (var 0)))).
+Definition inBool (n : nat) (t : Tm): Tm := inr (inr (inl t)).
 
-Lemma inBoolT {Γ n} : ⟪ Γ ⊢ inBool n : tbool ⇒ UVal (S n) ⟫.
+Lemma inBoolT {Γ n t} : ⟪ Γ ⊢ t : tbool ⟫ → ⟪ Γ ⊢ inBool n t : UVal (S n) ⟫.
 Proof.
   unfold inBool. crushTyping.
 Qed.
 
-Definition inProd (n : nat) : Tm := abs (UVal n × UVal n) (inr (inr (inr (inl (var 0))))).
+Definition inProd (n : nat) (t : Tm) : Tm := inr (inr (inr (inl t))).
 
-Lemma inProd_T {Γ n} : ⟪ Γ ⊢ inProd n : (UVal n × UVal n) ⇒ UVal (S n) ⟫.
+Lemma inProd_T {Γ n t} : ⟪ Γ ⊢ t : UVal n × UVal n ⟫ → ⟪ Γ ⊢ inProd n t : UVal (S n) ⟫.
 Proof.
   unfold inProd. crushTyping.
 Qed.
 
-Definition inArr (n : nat) : Tm := abs (UVal n ⇒ UVal n) (inr (inr (inr (inr (inl (var 0)))))).
+Definition inArr (n : nat) (t : Tm) : Tm := inr (inr (inr (inr (inl t)))).
 
-Lemma inArr_T {Γ n} : ⟪ Γ ⊢ inArr n : (UVal n ⇒ UVal n) ⇒ UVal (S n) ⟫.
+Lemma inArr_T {Γ n t} : ⟪ Γ ⊢ t : UVal n ⇒ UVal n ⟫ → ⟪ Γ ⊢ inArr n t : UVal (S n) ⟫.
 Proof.
   unfold inArr. crushTyping.
 Qed.
 
-Definition inSum (n : nat) : Tm := abs (UVal n ⊎ UVal n) (inr (inr (inr (inr (inr (var 0)))))).
+Definition inSum (n : nat) (t : Tm) : Tm := inr (inr (inr (inr (inr t)))).
 
-Lemma inSum_T {Γ n} : ⟪ Γ ⊢ inSum n : (UVal n ⊎ UVal n) ⇒ UVal (S n) ⟫.
+Lemma inSum_T {Γ n t} : ⟪ Γ ⊢ t : UVal n ⊎ UVal n ⟫ → ⟪ Γ ⊢ inSum n t : UVal (S n) ⟫.
 Proof.
   unfold inSum. crushTyping.
 Qed.
 
 
-(* Local Variables: *)
-(* coq-load-path: (("." "UVal") ("../Stlc" "Stlc")) *)
-(* End: *)
